proof/client.v
@@ -1,6 +1,6 @@
 From New.proof.github_com.sanjit_bhat.pav.client_proof Require Export
-  base client evidence.
+  base client.
 
 Module Import client.
-  Export base.client client.client evidence.client.
+  Export base.client client.client.
 End client.
