proof/ktcore.v
@@ -1,6 +1,6 @@
 From New.proof.github_com.sanjit_bhat.pav.ktcore_proof Require Export
-  base ktcore serde.
+  base evidence ktcore serde sigpred.
 
 Module Import ktcore.
-  Export base.ktcore ktcore.ktcore serde.ktcore.
+  Export base.ktcore evidence.ktcore ktcore.ktcore serde.ktcore sigpred.ktcore.
 End ktcore.
