proof/ktcore_proof/evidence.v
@@ -1,0 +1,328 @@
+From New.generatedproof.github_com.sanjit_bhat.pav Require Import ktcore.
+From New.proof.github_com.sanjit_bhat.pav Require Import prelude.
+
+From New.proof Require Import bytes.
+From New.proof.github_com.sanjit_bhat.pav Require Import
+  cryptoffi safemarshal.
+
+From New.proof.github_com.sanjit_bhat.pav.ktcore_proof Require Import
+  base ktcore serde sigpred.
+
+Module ktcore.
+Import ktcore.ktcore serde.ktcore sigpred.ktcore.
+
+Module EvidVrf.
+Record t :=
+  mk' {
+    VrfPk0: list w8;
+    Sig0: list w8;
+    VrfPk1: list w8;
+    Sig1: list w8;
+  }.
+
+Section proof.
+Context `{hG: heapGS Σ, !ffi_semantics _ _, !globalsGS Σ} {go_ctx : GoContext}.
+
+Definition own ptr obj d : iProp Σ :=
+  ∃ sl_VrfPk0 sl_Sig0 sl_VrfPk1 sl_Sig1,
+  "Hstruct" ∷ ptr ↦{d} (ktcore.EvidVrf.mk sl_VrfPk0 sl_Sig0 sl_VrfPk1 sl_Sig1) ∗
+
+  "Hsl_VrfPk0" ∷ sl_VrfPk0 ↦*{d} obj.(VrfPk0) ∗
+  "Hsl_Sig0" ∷ sl_Sig0 ↦*{d} obj.(Sig0) ∗
+  "Hsl_VrfPk1" ∷ sl_VrfPk1 ↦*{d} obj.(VrfPk1) ∗
+  "Hsl_Sig1" ∷ sl_Sig1 ↦*{d} obj.(Sig1).
+
+End proof.
+End EvidVrf.
+
+Module EvidLink.
+Record t :=
+  mk' {
+    Epoch: w64;
+    Link0: list w8;
+    Sig0: list w8;
+    Link1: list w8;
+    Sig1: list w8;
+  }.
+
+Section proof.
+Context `{hG: heapGS Σ, !ffi_semantics _ _, !globalsGS Σ} {go_ctx : GoContext}.
+
+Definition own ptr obj d : iProp Σ :=
+  ∃ sl_Link0 sl_Sig0 sl_Link1 sl_Sig1,
+  "Hstruct" ∷ ptr ↦{d} (ktcore.EvidLink.mk obj.(Epoch) sl_Link0 sl_Sig0 sl_Link1 sl_Sig1) ∗
+
+  "Hsl_Link0" ∷ sl_Link0 ↦*{d} obj.(Link0) ∗
+  "Hsl_Sig0" ∷ sl_Sig0 ↦*{d} obj.(Sig0) ∗
+  "Hsl_Link1" ∷ sl_Link1 ↦*{d} obj.(Link1) ∗
+  "Hsl_Sig1" ∷ sl_Sig1 ↦*{d} obj.(Sig1).
+
+End proof.
+End EvidLink.
+
+Module Evid.
+Record t :=
+  mk' {
+    Vrf: option EvidVrf.t;
+    Link: option EvidLink.t;
+  }.
+
+Section proof.
+Context `{hG: heapGS Σ, !ffi_semantics _ _, !globalsGS Σ} {go_ctx : GoContext}.
+
+Definition own ptr obj d : iProp Σ :=
+  ∃ ptr_Vrf ptr_Link,
+  "Hstruct" ∷ ptr ↦{d} (ktcore.Evid.mk ptr_Vrf ptr_Link) ∗
+
+  "Hown_Vrf" ∷
+    match obj.(Vrf) with
+    | Some Vrf => EvidVrf.own ptr_Vrf Vrf d
+    | None => ⌜ptr_Vrf = null⌝
+    end ∗
+  "Hown_Link" ∷
+    match obj.(Link) with
+    | Some Link => EvidLink.own ptr_Link Link d
+    | None => ⌜ptr_Link = null⌝
+    end.
+
+End proof.
+End Evid.
+
+Section proof.
+Context `{hG: heapGS Σ, !ffi_semantics _ _, !globalsGS Σ} {go_ctx : GoContext}.
+Context `{pavG Σ}.
+
+Definition wish_EvidVrf e pk : iProp Σ :=
+  "#Hwish0" ∷ wish_VrfSig pk e.(EvidVrf.VrfPk0) e.(EvidVrf.Sig0) ∗
+  "#Hwish1" ∷ wish_VrfSig pk e.(EvidVrf.VrfPk1) e.(EvidVrf.Sig1) ∗
+  "%Heq" ∷ ⌜e.(EvidVrf.VrfPk0) ≠ e.(EvidVrf.VrfPk1)⌝.
+
+Lemma wish_EvidVrf_sig_pred e pk γ :
+  wish_EvidVrf e pk -∗
+  ¬ cryptoffi.is_sig_pk pk (sigpred γ).
+Proof.
+  iIntros "@ #His_pk".
+  iNamedSuffix "Hwish0" "0".
+  iNamedSuffix "Hwish1" "1".
+  iDestruct (cryptoffi.is_sig_to_pred with "His_pk His_sig0") as "#HP0".
+  iDestruct (cryptoffi.is_sig_to_pred with "His_pk His_sig1") as "#HP1".
+  iDestruct "HP0" as "[H|H]"; [|by iNamed "H"].
+  iNamedSuffix "H" "0".
+  iDestruct "HP1" as "[H|H]"; [|by iNamed "H"].
+  iNamedSuffix "H" "1".
+  remember (VrfSig.mk' _ _) as o0 in Henc0.
+  remember (VrfSig.mk' _ _) as o1 in Henc0.
+  opose proof (VrfSig.wish_det [] [] o0 o1 _ _) as [? _].
+  { by list_simplifier. }
+  { rewrite /VrfSig.wish.
+    list_simplifier.
+    intuition.
+    by f_equal. }
+  remember (VrfSig.mk' _ _) as o2 in Henc1.
+  remember (VrfSig.mk' _ _) as o3 in Henc1.
+  opose proof (VrfSig.wish_det [] [] o2 o3 _ _) as [? _].
+  { by list_simplifier. }
+  { rewrite /VrfSig.wish.
+    list_simplifier.
+    intuition.
+    by f_equal. }
+  iCombine "Hshot0 Hshot1" gives %[_ <-].
+  simplify_eq/=.
+Qed.
+
+Lemma wp_EvidVrf_check ptr_e e sl_pk pk :
+  {{{
+    is_pkg_init ktcore ∗
+    "#Hown_evid" ∷ EvidVrf.own ptr_e e (□) ∗
+    "#Hsl_pk" ∷ sl_pk ↦*□ pk
+  }}}
+  ptr_e @ (ptrT.id ktcore.EvidVrf.id) @ "check" #sl_pk
+  {{{
+    (err : bool), RET #err;
+    "Hgenie" ∷
+      match err with
+      | true => ¬ wish_EvidVrf e pk
+      | false =>
+        "#Hwish_EvidVrf" ∷ wish_EvidVrf e pk
+      end
+  }}}.
+Proof.
+  wp_start as "@".
+  iNamed "Hown_evid".
+  wp_auto.
+  wp_apply wp_VerifyVrfSig as "* @".
+  { iFrame "#". }
+  wp_if_destruct.
+  { iApply "HΦ". iIntros "@". by iApply "Hgenie". }
+  iNamedSuffix "Hgenie" "0".
+  wp_apply wp_VerifyVrfSig as "* @".
+  { iFrame "#". }
+  wp_if_destruct.
+  { iApply "HΦ". iIntros "@". by iApply "Hgenie". }
+  iNamedSuffix "Hgenie" "1".
+  wp_apply bytes.wp_Equal as "_".
+  { iFrame "#". }
+  iApply "HΦ".
+  case_bool_decide.
+  - by iIntros "@".
+  - by iFrame "#".
+Qed.
+
+Definition wish_EvidLink e pk : iProp Σ :=
+  "#Hwish0" ∷ wish_LinkSig pk e.(EvidLink.Epoch) e.(EvidLink.Link0) e.(EvidLink.Sig0) ∗
+  "#Hwish1" ∷ wish_LinkSig pk e.(EvidLink.Epoch) e.(EvidLink.Link1) e.(EvidLink.Sig1) ∗
+  "%Heq" ∷ ⌜e.(EvidLink.Link0) ≠ e.(EvidLink.Link1)⌝.
+
+Lemma wish_EvidLink_sig_pred e pk γ :
+  wish_EvidLink e pk -∗
+  ¬ cryptoffi.is_sig_pk pk (sigpred γ).
+Proof.
+  iIntros "@ #His_pk".
+  destruct e. simpl in *.
+  iNamedSuffix "Hwish0" "0".
+  iNamedSuffix "Hwish1" "1".
+  iDestruct (cryptoffi.is_sig_to_pred with "His_pk His_sig0") as "#HP0".
+  iDestruct (cryptoffi.is_sig_to_pred with "His_pk His_sig1") as "#HP1".
+  iDestruct "HP0" as "[H|H]"; [by iNamed "H"|].
+  iNamedSuffix "H" "0".
+  iDestruct "HP1" as "[H|H]"; [by iNamed "H"|].
+  iNamedSuffix "H" "1".
+  remember (LinkSig.mk' _ _ _) as o0 in Henc0.
+  remember (LinkSig.mk' _ _ _) as o1 in Henc0.
+  opose proof (LinkSig.wish_det [] [] o0 o1 _ _) as [? _].
+  { by list_simplifier. }
+  { rewrite /LinkSig.wish.
+    list_simplifier.
+    intuition.
+    by f_equal. }
+  remember (LinkSig.mk' _ _ _) as o2 in Henc1.
+  remember (LinkSig.mk' _ _ _) as o3 in Henc1.
+  opose proof (LinkSig.wish_det [] [] o2 o3 _ _) as [? _].
+  { by list_simplifier. }
+  { rewrite /LinkSig.wish.
+    list_simplifier.
+    intuition.
+    by f_equal. }
+  simplify_eq/=.
+  iCombine "Hshot0 Hshot1" gives %[_ <-].
+  iDestruct (mono_list_idx_own_get with "Hlb0") as "Hidx0"; [done|].
+  iDestruct (mono_list_idx_own_get with "Hlb1") as "Hidx1"; [done|].
+  iDestruct (mono_list_idx_agree with "Hidx0 Hidx1") as %->.
+  done.
+Qed.
+
+Lemma wp_EvidLink_check ptr_e e sl_pk pk :
+  {{{
+    is_pkg_init ktcore ∗
+    "#Hown_evid" ∷ EvidLink.own ptr_e e (□) ∗
+    "#Hsl_pk" ∷ sl_pk ↦*□ pk
+  }}}
+  ptr_e @ (ptrT.id ktcore.EvidLink.id) @ "check" #sl_pk
+  {{{
+    (err : bool), RET #err;
+    "Hgenie" ∷
+      match err with
+      | true => ¬ wish_EvidLink e pk
+      | false =>
+        "#Hwish_EvidLink" ∷ wish_EvidLink e pk
+      end
+  }}}.
+Proof.
+  wp_start as "@".
+  iNamed "Hown_evid".
+  wp_auto.
+  wp_apply wp_VerifyLinkSig as "* @".
+  { iFrame "#". }
+  wp_if_destruct.
+  { iApply "HΦ". iIntros "@". by iApply "Hgenie". }
+  iNamedSuffix "Hgenie" "0".
+  wp_apply wp_VerifyLinkSig as "* @".
+  { iFrame "#". }
+  wp_if_destruct.
+  { iApply "HΦ". iIntros "@". by iApply "Hgenie". }
+  iNamedSuffix "Hgenie" "1".
+  wp_apply bytes.wp_Equal as "_".
+  { iFrame "#". }
+  iApply "HΦ".
+  case_bool_decide.
+  - by iIntros "@".
+  - by iFrame "#".
+Qed.
+
+Definition wish_Evid e pk : iProp Σ :=
+  match e.(Evid.Vrf), e.(Evid.Link) with
+  | Some e', None => wish_EvidVrf e' pk
+  | None, Some e' => wish_EvidLink e' pk
+  | _, _ => False
+  end.
+
+Lemma wish_Evid_sig_pred e pk γ :
+  wish_Evid e pk -∗
+  ¬ cryptoffi.is_sig_pk pk (sigpred γ).
+Proof.
+  iIntros "#Hwish #His_pk".
+  destruct e.
+  destruct Vrf as [Vrf|], Link as [Link|]; try done.
+  - iNamed "Hwish".
+    iApply (wish_EvidVrf_sig_pred Vrf); [|done].
+    by iFrame "#".
+  - iNamed "Hwish".
+    iApply (wish_EvidLink_sig_pred Link); [|done].
+    by iFrame "#".
+Qed.
+
+Lemma wp_Evid_Check ptr_e e sl_pk pk :
+  {{{
+    is_pkg_init ktcore ∗
+    "#Hown_evid" ∷ Evid.own ptr_e e (□) ∗
+    "#Hsl_pk" ∷ sl_pk ↦*□ pk
+  }}}
+  ptr_e @ (ptrT.id ktcore.Evid.id) @ "Check" #sl_pk
+  {{{
+    (err : bool), RET #err;
+    "Hgenie" ∷
+      match err with
+      | true => ¬ wish_Evid e pk
+      | false =>
+        "#Hwish_Evid" ∷ wish_Evid e pk
+      end
+  }}}.
+Proof.
+  wp_start as "@".
+  iNamed "Hown_evid".
+  wp_auto.
+  destruct e. simpl.
+
+  wp_if_destruct.
+  2: {
+    destruct Vrf.
+    2: { by iDestruct "Hown_Vrf" as %?. }
+    wp_if_destruct.
+    2: {
+      destruct Link.
+      2: { by iDestruct "Hown_Link" as %?. }
+      by iApply "HΦ". }
+    destruct Link.
+    { iNamedSuffix "Hown_Link" "'".
+      by iDestruct (typed_pointsto_not_null with "Hstruct'") as %?. }
+    wp_apply wp_EvidVrf_check as "* @".
+    { iFrame "#". }
+    by iApply "HΦ". }
+
+  destruct Vrf.
+  { iNamedSuffix "Hown_Vrf" "'".
+    by iDestruct (typed_pointsto_not_null with "Hstruct'") as %?. }
+  wp_if_destruct.
+  { destruct Link.
+    { iNamedSuffix "Hown_Link" "'".
+      by iDestruct (typed_pointsto_not_null with "Hstruct'") as %?. }
+    by iApply "HΦ". }
+  destruct Link.
+  2: { by iDestruct "Hown_Link" as %?. }
+  wp_apply wp_EvidLink_check as "* @".
+  { iFrame "#". }
+  by iApply "HΦ".
+Qed.
+
+End proof.
+End ktcore.
